Move some code into appropriate library locations, to support a nice short BabyThreadDriver safety proof

platform/tests/BabyThreadDriver.v
@@ -1,68 +1,20 @@
 Require Import Thread BabyThread Bootstrap.
 
 
-Notation "'bfunctionNoRet' name () [ p ] b 'end'" :=
-  (let p' := p in
-   let vars := nil in
-   let b' := b%SP in
-    {| FName := name;
-      FPrecondition := Precondition p' None;
-      FBody := ((fun _ _ =>
-        Structured nil (fun im mn _ => Structured.Assert_ im mn (Precondition p' (Some vars))));;
-      (fun ns res => b' ns (res - (List.length vars - List.length (Formals p')))%nat))%SP;
-      FVars := vars;
-      FReserved := Reserved p' |})
-  (no associativity, at level 95, name at level 0, p at level 0, only parsing) : SPfuncs_scope.
-
 Section boot.
   Variables heapSize : nat.
 
   Hypothesis heapSizeLowerBound : (3 <= heapSize)%nat.
-  Hypothesis heapSizeUpperBound : goodSize (4 * heapSize).
 
-  Lemma goodSize_heapSize : goodSize heapSize.
-    eapply goodSize_weaken; [ eassumption | omega ].
+  Definition size := heapSize + 50.
+
+  Hypothesis mem_size : goodSize (size * 4)%nat.
+
+  Let heapSizeUpperBound : goodSize (heapSize * 4).
+    unfold size in *; eapply goodSize_weaken; [ eassumption | omega ].
   Qed.
 
-  Hint Immediate goodSize_heapSize.
-
-  Theorem heapSizeLowerBound' : natToW 3 <= natToW heapSize.
-    intro; pre_nomega.
-    rewrite wordToNat_natToWord_idempotent in *.
-    rewrite wordToNat_natToWord_idempotent in *.
-    omega.
-    reflexivity.
-    change (goodSize heapSize); eapply goodSize_weaken; [ eassumption | omega ].
-  Qed.
-
-  Hint Immediate heapSizeLowerBound'.
-
-  Theorem noWrap : noWrapAround (natToW (0 + 4)) (wordToNat (natToW heapSize) - 1).
-    simpl; hnf; intros.
-    intro.
-    rewrite <- natToW_plus in H0.
-    apply natToW_inj in H0.
-    omega.
-    2: reflexivity.
-    rewrite wordToNat_natToWord_idempotent in *.
-    eapply goodSize_weaken; [ eassumption | omega ].
-    change (goodSize heapSize); eauto.
-  Qed.
-
-  Hint Extern 1 (noWrapAround _ _) => apply noWrap.
-
-  Theorem heapSize_roundTrip : wordToNat (natToW heapSize) = heapSize.
-    intros; apply wordToNat_natToWord_idempotent;
-      change (goodSize heapSize); eauto.
-  Qed.
-
-  Hint Rewrite heapSize_roundTrip : sepFormula.
-
-  Definition bootS := {|
-    Reserved := 49;
-    Formals := nil;
-    Precondition := fun _ => st ~> ![ 0 =?> (heapSize + 50) ] st
-  |}.
+  Definition bootS := bootS heapSize.
 
   Definition boot := bimport [[ "malloc"!"init" @ [Malloc.initS], "test"!"main" @ [BabyThread.mainS] ]]
     bmodule "main" {{
@@ -81,85 +33,9 @@ Section boot.
       end
     }}.
 
-  Lemma create_stack : forall ns ss sp,
-    NoDup ns
-    -> sp =?> (length ns + ss) ===> Ex vs, locals ns vs ss sp.
-    intros; eapply Himp_trans; [ apply allocated_split | ].
-    instantiate (1 := length ns); omega.
-    eapply Himp_trans.
-    eapply Himp_star_frame.
-    apply behold_the_array; auto.
-    apply Himp_refl.
-    unfold locals, array.
-    Opaque mult.
-    sepLemma.
-    apply allocated_shift_base.
-    Require Import Arith.
-    unfold natToW; rewrite mult_comm; words.
-    omega.
-  Qed.
-
-  Theorem genesis :
-    0 =?> (heapSize + 50)
-    ===> (Ex vs, locals ("rp" :: nil) vs 49 (heapSize * 4)%nat) * 0 =?> heapSize.
-    descend; intros; eapply Himp_trans; [ apply allocated_split | ].
-    instantiate (1 := heapSize); auto.
-    apply Himp_trans with (0 =?> heapSize *
-      (heapSize * 4)%nat =?> 50)%Sep.
-    apply Himp_star_frame.
-    apply Himp_refl.
-    apply allocated_shift_base.
-    Require Import Arith.
-    rewrite mult_comm.
-    simpl.
-    unfold natToW.
-    words.
-    omega.
-    apply Himp_trans with (0 =?> heapSize *
-      Ex vs, locals ("rp" :: nil) vs 49 (heapSize * 4)%nat)%Sep.
-    apply Himp_star_frame.
-    apply Himp_refl.
-    change 50 with (length ("rp" :: nil) + 49).
-    apply create_stack.
-    NoDup.
-    sepLemma.
-  Qed.
-
-  Transparent mult.
-
-  Definition genesisHints : TacPackage.
-    prepare genesis tt.
-  Defined.
-
   Theorem ok : moduleOk boot.
-    vcgen; abstract sep genesisHints.
+    vcgen; abstract (sep genesisHints; eauto).
   Qed.
-
-  Ltac link_simp := simpl Imports; simpl Exports;
-    cbv beta iota zeta delta [importsOk LabelMap.fold LabelMap.Raw.fold
-      LabelMap.this importsMap fold_left LabelMap.add LabelMap.Raw.add
-      LabelMap.empty LabelMap.Raw.empty
-      LabelKey.compare LabelKey.compare' string_lt
-      fst snd string_dec sumbool_rec sumbool_rect
-      Ascii.N_of_ascii Ascii.N_of_digits N.compare Pos.compare
-      string_rec string_rect Ascii.ascii_dec
-      LabelMap.find LabelMap.Raw.find Nplus Nmult Pos.compare_cont
-      Pos.add Pos.mul Ascii.ascii_rec Ascii.ascii_rect
-      Bool.bool_dec bool_rec bool_rect eq_rec_r eq_rec eq_rect eq_sym
-      label'_lt label'_eq label'_rec label'_rect
-      LabelMap.Raw.bal LabelMap.Raw.create
-      Int.Z_as_Int.gt_le_dec Int.Z_as_Int.plus Int.Z_as_Int.ge_lt_dec
-      LabelMap.Raw.height
-      ZArith_dec.Z_gt_le_dec Int.Z_as_Int._0
-      BinInt.Z.add Int.Z_as_Int._1 Int.Z_as_Int._2
-      ZArith_dec.Z_gt_dec ZArith_dec.Z_ge_lt_dec Int.Z_as_Int.max
-      BinInt.Z.max BinInt.Z.compare union ZArith_dec.Z_ge_dec
-      diff LabelMap.mem LabelMap.Raw.mem LabelMap.is_empty
-      LabelMap.Raw.is_empty Pos.succ].
-
-  Ltac link m1 m2 :=
-    apply linkOk; [ apply m1 | apply m2 | exact (refl_equal true)
-      | link_simp; tauto | link_simp; tauto | link_simp; tauto ].
 
   Definition m0 := link Malloc.m boot.
   Definition m1 := link Queue.m m0.
@@ -199,17 +75,8 @@ Section boot.
 
   Variable st : state.
 
-  Definition size := heapSize + 50.
-
-  Hypothesis mem_low : forall n, (n < 4 * size)%nat -> st.(Mem) n <> None.
-  Hypothesis mem_high : forall w, $(4 * size) <= w -> st.(Mem) w = None.
-  Hypothesis mem_size : goodSize (4 * size)%nat.
-
-  Ltac safety ok :=
-    eapply XCAP.safety; try apply ok; try eassumption; [
-      reflexivity
-      | apply LabelMap.find_2; link_simp; reflexivity
-      | propxFo; descend; apply materialize_allocated; assumption ].
+  Hypothesis mem_low : forall n, (n < size * 4)%nat -> st.(Mem) n <> None.
+  Hypothesis mem_high : forall w, $(size * 4) <= w -> st.(Mem) w = None.
 
   Theorem safe : safe stn prog (w, st).
     safety ok3.
