platform/Scheduler.v
@@ -1,4 +1,4 @@
-Require Import AutoSep Bags Malloc Queue.
+Require Import Arith AutoSep Bags Malloc Queue.
 
 Set Implicit Arguments.
 
@@ -101,26 +101,6 @@ End Sched.
 Import Sched.
 Export Sched.
 Hint Immediate sched_extensional.
-
-Lemma create_stack : forall ns ss sp,
-  NoDup ns
-  -> sp =?> (length ns + ss) ===> Ex vs, locals ns vs ss sp.
-  intros; eapply Himp_trans; [ apply allocated_split | ].
-  instantiate (1 := length ns); omega.
-  eapply Himp_trans.
-  eapply Himp_star_frame.
-  apply behold_the_array; auto.
-  apply Himp_refl.
-  unfold locals, array.
-  Opaque mult.
-  sepLemma.
-  apply allocated_shift_base.
-  Require Import Arith.
-  unfold natToW; rewrite mult_comm; words.
-  omega.
-Qed.
-
-Transparent mult.
 
 Definition hints : TacPackage.
   prepare (sched_fwd, create_stack) (sched_bwd, susps_empty_bwd, susps_add_bwd).
